x86/LinkingC2.v
@@ -1,0 +1,120 @@
+Require Import Coqlib Maps Errors AST Linking LinkingC sflib.
+
+Remark link_transf_partial_fundef_rev:
+  forall (A B: Type) (tr1 tr2: A -> res B) (f1 f2: fundef A) (tf1 tf2: fundef B) (tf: fundef B),
+  link tf1 tf2 = Some tf ->
+  transf_partial_fundef tr1 f1 = OK tf1 ->
+  transf_partial_fundef tr2 f2 = OK tf2 ->
+  exists f,
+      link f1 f2 = Some f
+  /\ (transf_partial_fundef tr1 f = OK tf \/ transf_partial_fundef tr2 f = OK tf).
+Proof.
+  Local Transparent Linker_fundef.
+  ss; ii. destruct f1, f2; ss; monadInv H0; monadInv H1.
+  - discriminate.
+  - destruct e; clarify. esplits; eauto. ss. rewrite EQ. ss. clarify. eauto.
+  - destruct e; clarify. esplits; eauto. ss. rewrite EQ. ss. clarify. eauto.
+  - destruct (external_function_eq e e0); clarify; inv H; des_ifs. eauto.
+Qed.
+
+Instance TransfPartialContextualLink_rev
+           {A B C V: Type} {LV: Linker V}
+           (tr_fun: C -> A -> res B)
+           (ctx_for: program (fundef B) V -> C):
+  TransfLink (fun (p2: program (fundef B) V) (p1: program (fundef A) V) =>
+              match_program
+                (fun cu tf f => AST.transf_partial_fundef (tr_fun (ctx_for cu)) f = OK tf)
+                eq p2 p1).
+Proof.
+  red. intros. destruct (link_linkorder _ _ _ H) as [LO1 LO2].
+  eapply link_match_program; eauto.
+- intros. eapply link_transf_partial_fundef_rev; eauto.
+- intros; subst. exists v; auto.
+Qed.
+
+Instance TransfPartialLink_rev
+           {A B V: Type} {LV: Linker V}
+           (tr_fun: A -> res B):
+  TransfLink (fun (p2: program (fundef B) V) (p1: program (fundef A) V) =>
+              match_program
+                (fun cu tf f => AST.transf_partial_fundef tr_fun f = OK tf)
+                eq p2 p1).
+Proof.
+  red. intros. destruct (link_linkorder _ _ _ H) as [LO1 LO2].
+  eapply link_match_program; eauto.
+- intros. eapply link_transf_partial_fundef_rev; eauto.
+- intros; subst. exists v; auto.
+Qed.
+
+Instance TransfTotallContextualLink_rev
+           {A B C V: Type} {LV: Linker V}
+           (tr_fun: C -> A -> B)
+           (ctx_for: program (fundef B) V -> C):
+  TransfLink (fun (p2: program (fundef B) V) (p1: program (fundef A) V) =>
+              match_program
+                (fun cu tf f => tf = AST.transf_fundef (tr_fun (ctx_for cu)) f)
+                eq p2 p1).
+Proof.
+  red. intros. destruct (link_linkorder _ _ _ H) as [LO1 LO2].
+  eapply link_match_program; eauto.
+- intros. subst. destruct tf1, tf2; simpl in *.
++ discriminate.
++ destruct e; inv H2. econstructor; eauto.
++ destruct e; inv H2. econstructor; eauto.
++ destruct (external_function_eq e e0); inv H2. econstructor; eauto.
+- intros; subst. exists v; auto.
+Qed.
+
+Instance TransfTotalLink_rev
+           {A B V: Type} {LV: Linker V}
+           (tr_fun: A -> B):
+  TransfLink (fun (p2: program (fundef B) V) (p1: program (fundef A) V) =>
+              match_program
+                (fun cu tf f => tf = AST.transf_fundef tr_fun f)
+                eq p2 p1).
+Proof.
+  red. intros. destruct (link_linkorder _ _ _ H) as [LO1 LO2].
+  eapply link_match_program; eauto.
+- intros. subst. destruct tf1, tf2; simpl in *.
++ discriminate.
++ destruct e; inv H2. econstructor; eauto.
++ destruct e; inv H2. econstructor; eauto.
++ destruct (external_function_eq e e0); inv H2. econstructor; eauto.
+- intros; subst. exists v; auto.
+Qed.
+
+
+Section LINK_LIST_MATCH.
+
+  Context {A B: Type} {LA: Linker A} {LB: Linker B} (prog_match: A -> B -> Prop) {TL: TransfLink prog_match}.
+
+  Theorem link_list_aux_match al bl
+          (MATCH:list_forall2 prog_match al bl)
+    :
+      forall a (SUCCESS: link_list_aux al = success a),
+      exists b, link_list_aux bl = success b /\ prog_match a b.
+  Proof.
+    revert bl MATCH.
+    induction al; ss; i; ss; inv MATCH; ss.
+    destruct (link_list_aux al) eqn:EQ; clarify.
+    - assert (al = []).
+      { destruct al; ss.
+        des_ifs. }
+      clarify. inv H3. ss. eauto.
+    - des_ifs_safe.
+      exploit IHal; eauto. i. des. rewrite H.
+      exploit TL; eauto. i. des. rewrite H2. eauto.
+  Qed.
+
+  Theorem link_list_match al bl
+          (MATCH:list_forall2 prog_match al bl)
+    :
+      forall a, link_list al = Some a ->
+                exists b, link_list bl = Some b /\ prog_match a b.
+  Proof.
+    i. unfold link_list in *. des_ifs_safe.
+    exploit link_list_aux_match; eauto.
+    i. des. rewrite H. eauto.
+  Qed.
+
+End LINK_LIST_MATCH.
